AbstractInterpreter.v
@@ -59,8 +59,9 @@ Definition eval_if_abstract {S A} `{Joinable S, Joinable A}
 Definition eval_catch_abstract {S A} `{Joinable S, Joinable A} 
   (st1 st2 : State S A) : State S A :=
   fun st => match (st1 st) with
-  | None => join_op st1 st2 st
-  | _ => st1 st
+  | (crashed _, st') => (crashed A, st')
+  | (failed _, st') => st2 st'
+  | x => x
   end.
 
 Fixpoint ceval_abstract (c : com) : State abstract_store unit :=
